Create some structure for stack_callProof

compiler/backend/proofs/stack_callProofScript.sml
@@ -6,19 +6,92 @@ open preamble stackLangTheory stackSemTheory stack_callTheory;
 
 val _ = new_theory("stack_callProof");
 
-Theorem dest_StackFree_thm
-  `dest_StackFree x = SOME  m <=> x = StackFree m`
-   (EQ_TAC
-     >- (Cases_on `x`
-          >> (fs[dest_StackFree_def]))
-     >> (fs[dest_StackFree_def]));
+Theorem dest_StackFree_SOME[simp]:
+  dest_StackFree x = SOME m <=> x = StackFree m
+Proof
+  Cases_on `x`
+  \\ fs[dest_StackFree_def]
+QED;
 
-Theorem dest_StackFree2_thm
-  `dest_StackFree x = NONE <=> !m. x <> StackFree m`
-  (EQ_TAC
-    >> (Cases_on `x`
-         >> (fs[dest_StackFree_def])));
+Theorem dest_StackFree_NONE[simp]:
+  dest_StackFree x = NONE <=> !m. x <> StackFree m
+Proof
+  Cases_on `x`
+  \\ fs[dest_StackFree_def]
+QED;
 
+val state_rel_def = Define `
+  state_rel s t <=>
+    t.clock = s.clock /\
+    t.regs = s.regs /\
+    t.stack = s.stack /\
+    t.stack_space = s.stack_space /\
+    ARB (* TODO: complete this *)`;
 
+val tree_accurate_def = Define `
+  tree_accurate tree (s_code:('a stackLang$prog) num_map) <=>
+    T (* TODO: for every entry in tree,
+                 there is code in s_code such that get_alloc for that
+                 code returns what is stored in the tree (in other words,
+                 tree is accurate w.r.t. s_code and get_alloc) *)`;
+
+(*
+  <| regs := dfgdg ; clock := 676 |> with clock := 3
+=
+  <| regs := dfgdg ; clock := 3 |>
+*)
+
+Theorem opt_code_correct:
+  !prog s res s1 t tree.
+    evaluate (prog,s) = (res,s1) /\ state_rel s t /\
+    tree_accurate tree s.code /\ res <> SOME Error ==>
+    ?ck t1. evaluate (opt_code prog tree,t with clock := t.clock + ck) =
+              (res,t1) /\ state_rel s1 t1 /\ tree_accurate tree s1.code
+Proof
+
+  recInduct evaluate_ind \\ rpt strip_tac
+  THEN1
+   (rename [`Skip`]
+    \\ fs [opt_code_def,evaluate_def] \\ rveq
+    \\ qexists_tac `0` \\ fs [state_rel_def])
+  THEN1
+   (rename [`Halt`]
+    \\ fs [opt_code_def,evaluate_def] \\ rveq
+    \\ fs [get_var_def,state_rel_def]
+    \\ TOP_CASE_TAC \\ fs []
+    \\ rveq \\ fs [empty_env_def])
+  THEN1 cheat
+  THEN1 cheat
+  THEN1 cheat
+  THEN1 cheat
+  THEN1 cheat
+  THEN1
+
+   (rename [`Seq p1 p2`]
+    \\ once_rewrite_tac [opt_code_def] \\ simp []
+    \\ TOP_CASE_TAC
+    THEN1
+     (fs [evaluate_def]
+      \\ Cases_on `evaluate (p1,s)` \\ fs []
+      \\ rename [`evaluate (p1,s) = (res0,s0)`]
+      \\ reverse (Cases_on `res0`)
+      THEN1
+       (fs [] \\ rveq \\ fs []
+        \\ first_x_assum (qspecl_then [`t`,`tree`] mp_tac)
+        \\ fs [] \\ strip_tac
+        \\ qexists_tac `ck` \\ fs [])
+      \\ fs []
+      \\ first_x_assum (qspecl_then [`t`,`tree`] mp_tac)
+      \\ fs [] \\ strip_tac
+      \\ first_x_assum (qspecl_then [`t1`,`tree`] mp_tac)
+      \\ fs [] \\ strip_tac
+      \\ qexists_tac `ck+ck'`
+      \\ qpat_x_assum `_ = (NONE,t1)` assume_tac
+      \\ drule (GEN_ALL stackPropsTheory.evaluate_add_clock)
+      \\ fs [])
+    \\ cheat)
+
+  \\ cheat
+QED;
 
 val _ = export_theory();
